rename: what we called `Wlp` in the code is `Wp`
In the paper submission we always called it `Wp`. This fixes the
confusion.

Veil/DSL/Action/Theory.lean
@@ -3,8 +3,8 @@ import Veil.DSL.Base
 /-!
   # Action Language
 
-  This file defines the syntax and semantics for the imperative language
-  we use to define initializers and actions.
+  This file defines the semantics for the imperative language we use to
+  define initializers and actions.
 -/
 section Veil
 open Classical
@@ -33,7 +33,7 @@ variable (m : Mode) (σ ρ : Type)
 @[inline] abbrev ActProp := σ -> σ -> Prop
 
 /- In Veil we will be using two different types of semantics:
-  - [Wlp]: Omni semantics, which relates a state `s : σ` to set of the
+  - [Wp]: Omni semantics, which relates a state `s : σ` to set of the
     possible program outcomes `post : RProp σ`
   - [BigStep]: Standard big-step semantics, which relates a state `s : σ`
     to a return value `r : ρ` and a post-state `s' : σ`
@@ -46,7 +46,7 @@ set_option linter.unusedVariables false in
     To model that we treat all `require` statements as `assert`'s.
   - `external` for enviorment calls. In this case envioremnt should provide a necessary conditions to
     satisfy all `require`'s. To model that we treat all `require` statements as `assume`'s. -/
-abbrev Wlp (m : Mode) (σ ρ : Type) := σ -> RProp σ ρ -> Prop
+abbrev Wp (m : Mode) (σ ρ : Type) := σ -> RProp σ ρ -> Prop
 /-- [BigStep]: Standard big-step semantics, which relates a state `s : σ` to a return value `r : ρ` and a post-state `s' : σ` -/
 abbrev BigStep := σ -> ρ -> σ -> Prop
 
@@ -57,9 +57,9 @@ section Theory
 
 variable {σ ρ : Type}
 
-/-! ### Relation between `BigStep` and `Wlp`  -/
+/-! ### Relation between `BigStep` and `Wp`  -/
 
-/-- `Wlp.toBigStep` converts Omni semantics to a Big-step one. Note that, it only
+/-- `Wp.toBigStep` converts Omni semantics to a Big-step one. Note that, it only
   makes sence is `act` terminates, in other words, the following holds
 
   ```∀ s, ∃ Q, act s Q```
@@ -73,28 +73,28 @@ variable {σ ρ : Type}
   send to the solver.
    -/
 @[actSimp]
-def Wlp.toBigStep {σ} (act : Wlp m σ ρ) : BigStep σ ρ :=
+def Wp.toBigStep {σ} (act : Wp m σ ρ) : BigStep σ ρ :=
   fun s r' s' =>
     act s (fun _ _ => True) ∧
     ¬ act s (fun r₀ s₀ => ¬ (r' = r₀ ∧ s' = s₀))
 
-/-- [BigStep.toWlp] converts Big-step semantics to Omni one.
+/-- [BigStep.toWp] converts Big-step semantics to Omni one.
 
   Ideally, here we should also assert termination of `act`, but this will be handled
   via `Sound` condition later. -/
 @[actSimp]
-def BigStep.toWlp {σ} (act : BigStep σ ρ) : Wlp .internal σ ρ :=
+def BigStep.toWp {σ} (act : BigStep σ ρ) : Wp .internal σ ρ :=
   fun s post => ∀ r s', act s r s' -> post r s'
 
 
-/-- Function which transforms any two-state formula into `Wlp` -/
+/-- Function which transforms any two-state formula into `Wp` -/
 @[actSimp]
-def Function.toWlp (m : Mode) (r : σ -> σ -> Prop) : Wlp m σ Unit :=
+def Function.toWp (m : Mode) (r : σ -> σ -> Prop) : Wp m σ Unit :=
   fun s post => ∀ s', r s s' -> post () s'
 
-/-- Function which transforms any `Wlp` into a two-state formula -/
+/-- Function which transforms any `Wp` into a two-state formula -/
 @[actSimp]
-def Wlp.toActProp {σ} (act : Wlp m σ ρ) : ActProp σ :=
+def Wp.toActProp {σ} (act : Wp m σ ρ) : ActProp σ :=
   fun s s' =>
     act s (fun _ _ => True) ∧
     ¬ act s (fun _ s₀ => ¬ (s' = s₀))
@@ -102,29 +102,29 @@ def Wlp.toActProp {σ} (act : Wlp m σ ρ) : ActProp σ :=
 /-! ### Languge statements -/
 
 @[actSimp]
-def Wlp.pure (r : ρ) : Wlp m σ ρ := fun s post => post r s
+def Wp.pure (r : ρ) : Wp m σ ρ := fun s post => post r s
 @[actSimp]
-def Wlp.bind (wp : Wlp m σ ρ) (wp_cont : ρ -> Wlp m σ ρ') : Wlp m σ ρ' :=
+def Wp.bind (wp : Wp m σ ρ) (wp_cont : ρ -> Wp m σ ρ') : Wp m σ ρ' :=
   fun s post => wp s (fun r s' => wp_cont r s' post)
 
 @[actSimp]
-def Wlp.assume (asm : Prop) : Wlp m σ PUnit := fun s post => asm → post () s
+def Wp.assume (asm : Prop) : Wp m σ PUnit := fun s post => asm → post () s
 @[actSimp]
-def Wlp.assert (ast : Prop) : Wlp m σ PUnit := fun s post => ast ∧ post () s
+def Wp.assert (ast : Prop) : Wp m σ PUnit := fun s post => ast ∧ post () s
 @[actSimp]
-def Wlp.fresh (τ : Type) : Wlp m σ τ := fun s post => ∀ t, post t s
+def Wp.fresh (τ : Type) : Wp m σ τ := fun s post => ∀ t, post t s
 
 @[actSimp]
-def Wlp.require (rq : Prop) : Wlp m σ PUnit :=
+def Wp.require (rq : Prop) : Wp m σ PUnit :=
   match m with
-  | Mode.internal => Wlp.assert rq
-  | Mode.external => Wlp.assume rq
+  | Mode.internal => Wp.assert rq
+  | Mode.external => Wp.assume rq
 
-/-- `Wlp.spec req ens` is the weakest precondition for a function with
+/-- `Wp.spec req ens` is the weakest precondition for a function with
   precondition `req` and postcondition `ens`.
 -/
 @[actSimp]
-def Wlp.spec (req : SProp σ) (ens : σ -> RProp σ ρ) : Wlp m σ ρ :=
+def Wp.spec (req : SProp σ) (ens : σ -> RProp σ ρ) : Wp m σ ρ :=
   fun s post =>
     match m with
     | .internal => req s ∧ ∀ r' s', (ens s r' s' -> post r' s')
@@ -136,42 +136,42 @@ def BigStep.spec (req : SProp σ) (ens : σ -> RProp σ ρ) : BigStep σ ρ :=
   fun s r s' => req s ∧ (req s -> ens s r s')
 
 @[actSimp]
-def Wlp.get : Wlp m σ σ := fun s post => post s s
+def Wp.get : Wp m σ σ := fun s post => post s s
 @[actSimp]
-def Wlp.set (s' : σ) : Wlp m σ Unit := fun _ post => post () s'
+def Wp.set (s' : σ) : Wp m σ Unit := fun _ post => post () s'
 @[actSimp]
-def Wlp.modifyGet (act : σ -> ρ × σ) : Wlp m σ ρ := fun s post => let (ret, s') := act s ; post ret s'
+def Wp.modifyGet (act : σ -> ρ × σ) : Wp m σ ρ := fun s post => let (ret, s') := act s ; post ret s'
 
 
 -- def BigStep.choice : BigStep σ ρ -> BigStep σ ρ -> BigStep σ ρ :=
 --   fun act act' s r s' => act s r s' ∨ act' s r s'
 
 /- BAD: it duplicates post -/
--- def Wlp.choice : Wlp σ ρ -> Wlp σ ρ -> Wlp σ ρ :=
+-- def Wp.choice : Wp σ ρ -> Wp σ ρ -> Wp σ ρ :=
 --   fun wp wp' s post => wp s post ∨ wp' s post
 
--- def Wlp.choice (wp : Wlp σ ρ) (wp' : Wlp σ ρ) : Wlp σ ρ :=
---   wp.toBigStep.choice wp'.toBigStep |>.toWlp
+-- def Wp.choice (wp : Wp σ ρ) (wp' : Wp σ ρ) : Wp σ ρ :=
+--   wp.toBigStep.choice wp'.toBigStep |>.toWp
 
 /-! ### Monad Instances -/
 
-instance : Monad (Wlp m σ) where
-  pure := Wlp.pure
-  bind := Wlp.bind
+instance : Monad (Wp m σ) where
+  pure := Wp.pure
+  bind := Wp.bind
 
-instance : MonadStateOf σ (Wlp m σ) where
-  get := Wlp.get
-  set := Wlp.set
-  modifyGet := Wlp.modifyGet
+instance : MonadStateOf σ (Wp m σ) where
+  get := Wp.get
+  set := Wp.set
+  modifyGet := Wp.modifyGet
 
-@[wlpSimp]
-def pureE : pure = Wlp.pure (σ := σ) (ρ := ρ) (m := m) := rfl
-@[wlpSimp]
-def bindE : bind = Wlp.bind (σ := σ) (ρ := ρ) (ρ' := ρ') (m := m) := rfl
-@[wlpSimp]
-def getE : get = Wlp.get (σ := σ) (m := m) := rfl
-@[wlpSimp]
-def modifyGetE : modifyGet = Wlp.modifyGet (σ := σ) (ρ := ρ) (m := m) := rfl
+@[wpSimp]
+def pureE : pure = Wp.pure (σ := σ) (ρ := ρ) (m := m) := rfl
+@[wpSimp]
+def bindE : bind = Wp.bind (σ := σ) (ρ := ρ) (ρ' := ρ') (m := m) := rfl
+@[wpSimp]
+def getE : get = Wp.get (σ := σ) (m := m) := rfl
+@[wpSimp]
+def modifyGetE : modifyGet = Wp.modifyGet (σ := σ) (ρ := ρ) (m := m) := rfl
 
 /-- `σ` is a sub-state of `σ'` -/
 class IsSubStateOf (σ : semiOutParam Type) (σ' : Type) where
@@ -186,26 +186,26 @@ class IsSubStateOf (σ : semiOutParam Type) (σ' : Type) where
 export IsSubStateOf (setIn getFrom)
 
 @[actSimp]
-def Wlp.lift {σ σ'} [IsSubStateOf σ σ'] (act : Wlp m σ ρ) : Wlp m σ' ρ :=
+def Wp.lift {σ σ'} [IsSubStateOf σ σ'] (act : Wp m σ ρ) : Wp m σ' ρ :=
   fun s' post => act (getFrom s') (fun r s => post r (setIn s s'))
 
-instance [IsSubStateOf σ σ'] : MonadLift (Wlp m σ) (Wlp m σ') where
-  monadLift := Wlp.lift
+instance [IsSubStateOf σ σ'] : MonadLift (Wp m σ) (Wp m σ') where
+  monadLift := Wp.lift
 
-@[wlpSimp]
-def monadLiftE [IsSubStateOf σ σ'] : monadLift = Wlp.lift (σ := σ) (σ' := σ') (ρ := ρ) (m := m) := rfl
+@[wpSimp]
+def monadLiftE [IsSubStateOf σ σ'] : monadLift = Wp.lift (σ := σ) (σ' := σ') (ρ := ρ) (m := m) := rfl
 
 /-! ### Lifting transitions -/
 
 /-- This theorem lets us lift a transition in a way that does not introduce
 quantification over `σ` in the lifted transition. -/
 theorem lift_transition {σ σ'} [IsSubStateOf σ σ'] (m : Mode) (r : σ -> σ -> Prop) :
-  (@Wlp.lift _  m σ σ' _ (r.toWlp m)).toActProp =
+  (@Wp.lift _  m σ σ' _ (r.toWp m)).toActProp =
   fun st st' =>
     r (getFrom st) (getFrom st') ∧
     st' = (setIn (@getFrom σ σ' _ st') st)
   := by
-  unfold Wlp.lift Function.toWlp Wlp.toActProp
+  unfold Wp.lift Function.toWp Wp.toActProp
   funext st st'
   simp only [implies_true, not_forall, not_imp, Decidable.not_not, true_and, eq_iff_iff]
   constructor
@@ -218,17 +218,17 @@ theorem lift_transition {σ σ'} [IsSubStateOf σ σ'] (m : Mode) (r : σ -> σ 
 
 /-! ### Soundness proof -/
 
-abbrev refines {σ ρ} (act : Wlp m σ ρ) (act' : Wlp m σ ρ) : Prop :=
+abbrev refines {σ ρ} (act : Wp m σ ρ) (act' : Wp m σ ρ) : Prop :=
   ∀ s post, act s post -> act' s post
 
-instance : LE (Wlp m σ ρ) where
+instance : LE (Wp m σ ρ) where
   le := refines
 
-abbrev Wlp.triple {σ ρ} (req : SProp σ) (act : Wlp m σ ρ) (ens : RProp σ ρ) : Prop :=
+abbrev Wp.triple {σ ρ} (req : SProp σ) (act : Wp m σ ρ) (ens : RProp σ ρ) : Prop :=
   ∀ s, req s -> act s ens
 
 /- Termination -/
-abbrev Wlp.terminates {σ } (req : SProp σ) (act : Wlp m σ ρ)  : Prop :=
+abbrev Wp.terminates {σ } (req : SProp σ) (act : Wp m σ ρ)  : Prop :=
   ∀ s, req s -> act s (fun _ _ => True)
 
 
@@ -239,7 +239,7 @@ abbrev ActProp.triple {σ } (req : SProp σ) (act : ActProp σ) (ens : SProp σ)
 
 
 /-- `Sound act` states the set of minimal conditions on `act` that are required
-  to prove the soundness of the `Wlp.toBigStep` conversion.
+  to prove the soundness of the `Wp.toBigStep` conversion.
   - first condition `inter` is a generalization of the following statement:
     ```lean
       ∀ s post post', act s post -> act s post' ->
@@ -254,14 +254,14 @@ abbrev ActProp.triple {σ } (req : SProp σ) (act : ActProp σ) (ens : SProp σ)
   - third condition `call`, states that the `internal` mode of `act` refines the `external`
     one. In other words, if you have proven some striple for `internal` mode of `act`,
     the same one holds for its `external` version -/
-class Sound {σ ρ : Type} (act : Wlp m σ ρ) where
+class Sound {σ ρ : Type} (act : Wp m σ ρ) where
   inter {τ : Type} [Inhabited τ] (post : τ -> RProp σ ρ) :
     ∀ s : σ, (∀ t : τ, act s (post t)) -> act s (∀ t, post t · ·)
   impl (post post' : RProp σ ρ) : ∀ s,
     (∀ r s, post r s -> post' r s) -> act s post -> act s post'
   -- call : act .internal <= act .external
 
-theorem sound_and (act : Wlp m σ ρ) [Sound act] :
+theorem sound_and (act : Wp m σ ρ) [Sound act] :
   act s post -> act s post' -> act s fun r s => post r s ∧ post' r s := by
   intro hact hact'
   let Post := fun (b : Bool) => if b then post' else post
@@ -274,10 +274,10 @@ theorem sound_and (act : Wlp m σ ρ) [Sound act] :
 --   have post_eq : post = (fun _ _ => Empty -> True) := by ext; simp_all
 --   rw [post_eq]; apply Sound.inter; rintro ⟨⟩
 
--- theorem wlp_sound (act : ∀ m, Wlp m σ ρ) [Sound act] :
---   ∀ s post, (act m).toBigStep.toWlp (m := m) s post <-> act m s post := by
+-- theorem wp_sound (act : ∀ m, Wp m σ ρ) [Sound act] :
+--   ∀ s post, (act m).toBigStep.toWp (m := m) s post <-> act m s post := by
 --   intro s post; constructor
---   { unfold Wlp.toBigStep BigStep.toWlp; simp
+--   { unfold Wp.toBigStep BigStep.toWp; simp
 --     intro hact
 --     have post_impl : ∀ r s, (∀ r' s', ¬ post r' s' -> ¬ (r' = r ∧ s' = s)) -> post r s := by
 --       intro r s impl
@@ -316,7 +316,7 @@ theorem triple_sound [Sound act] (req : SProp σ) (ens : SProp σ) :
 theorem triple_sound' [Sound act] (req : SProp σ) (ens : RProp σ ρ) :
   act.triple req ens → act.toActProp.triple req (∃ r, ens r ·) := by
   intro htriple s s' hreq ⟨_, hact⟩
-  unfold Wlp.triple at htriple
+  unfold Wp.triple at htriple
   specialize htriple _ hreq
   false_or_by_contra ; rename_i h ; simp at h
   apply hact ; apply Sound.impl (post := ens) <;> try assumption
@@ -333,62 +333,62 @@ theorem triple_sound'_ret_unit [Sound act] (req : SProp σ) (ens : RProp σ PUni
 theorem triple_sound'_ret_unit' [Sound act] {st : σ} (ens : RProp σ PUnit) :
   act st ens → (∀ st', act.toActProp st st' → ens () st') := by
   have h := triple_sound'_ret_unit (act := act) (fun stt => stt = st) ens
-  unfold Wlp.triple ActProp.triple at h ; simp at h
+  unfold Wp.triple ActProp.triple at h ; simp at h
   intro hq st' ; specialize h hq st st' rfl ; exact h
 
-instance pure_sound : Sound (Wlp.pure (σ := σ) (m := m) r) where
+instance pure_sound : Sound (Wp.pure (σ := σ) (m := m) r) where
   inter := by simp [pure, actSimp]
   impl  := by intros; simp_all [pure, actSimp]
   -- call  := by solve_by_elim
 
-instance bind_sound (act : Wlp m' σ ρ) (act' : ρ -> Wlp m σ ρ') [Sound act] [∀ r, Sound (act' r)] : Sound (Wlp.bind (m := m) act act') where
+instance bind_sound (act : Wp m' σ ρ) (act' : ρ -> Wp m σ ρ') [Sound act] [∀ r, Sound (act' r)] : Sound (Wp.bind (m := m) act act') where
   inter := by
-    unfold Wlp.bind
+    unfold Wp.bind
     intros τ _ post s hbind
     apply Sound.impl (∀ t, act' · · <| post t) <;> solve_by_elim [Sound.inter]
   impl := by
-    unfold Wlp.bind
+    unfold Wp.bind
     intros post post' s hpost hbind
     apply Sound.impl (act' · · <| post) <;> (intros; solve_by_elim [Sound.impl])
 
-instance (priority := low) internal_sound (act : Wlp m σ ρ) [inst : Sound (m := .internal) act] : Sound (m := .external) act where
+instance (priority := low) internal_sound (act : Wp m σ ρ) [inst : Sound (m := .internal) act] : Sound (m := .external) act where
   inter := inst.inter
   impl := inst.impl
 
   -- call := by
-  --   unfold Wlp.bind
+  --   unfold Wp.bind
   --   intros s post hbind
   --   apply Sound.call; apply Sound.impl;
   --   { intros _ _; apply Sound.call }
   --   solve_by_elim
 
-instance assume_sound : Sound (Wlp.assume (m := m) (σ := σ) rq) where
+instance assume_sound : Sound (Wp.assume (m := m) (σ := σ) rq) where
   inter := by intros; simp_all [actSimp]
   impl := by intros; simp_all [actSimp]
   -- call := by solve_by_elim
 
-instance assert_sound : Sound (Wlp.assert (m := m) (σ := σ) rq) where
+instance assert_sound : Sound (Wp.assert (m := m) (σ := σ) rq) where
   inter := by intros; simp_all [actSimp]; rename_i h; specialize h default; simp [*]
   impl  := by intros; simp_all [actSimp] <;> solve_by_elim
   -- call  := by solve_by_elim
 
-instance require_sound : Sound (Wlp.require (m := m) (σ := σ) rq) where
+instance require_sound : Sound (Wp.require (m := m) (σ := σ) rq) where
   inter := by
     cases m
     { intros; simp_all [actSimp]; rename_i h; specialize h default; simp [*] }
     intros; simp_all [actSimp]
   impl := by cases m <;> (intros; simp_all [actSimp] <;> solve_by_elim)
   -- call := by
-  --  intros s post; unfold Wlp.require; simp [Wlp.assert, Wlp.assume]; solve_by_elim
+  --  intros s post; unfold Wp.require; simp [Wp.assert, Wp.assume]; solve_by_elim
 
 
-instance fresh_sound : Sound (Wlp.fresh (m := m) (σ := σ) τ) where
+instance fresh_sound : Sound (Wp.fresh (m := m) (σ := σ) τ) where
   inter := by intros; simp_all [actSimp]
   impl := by intros; simp_all [actSimp]
   -- call := by solve_by_elim
 
 
-instance spec_sound : Sound (Wlp.spec (m := m) req ens) where
+instance spec_sound : Sound (Wp.spec (m := m) req ens) where
   inter := by
     cases m <;> (intros; simp_all [actSimp])
     rename_i h; intros; specialize h default; simp [*]
@@ -398,24 +398,24 @@ instance spec_sound : Sound (Wlp.spec (m := m) req ens) where
     solve_by_elim
   -- call := by intros _; simp_all [actSimp]
 
-instance (r : σ -> σ -> Prop) : Sound (r.toWlp (m := m)) where
+instance (r : σ -> σ -> Prop) : Sound (r.toWp (m := m)) where
   inter := by intros; simp_all [actSimp]
   impl := by intros; simp_all [actSimp]
   -- call := by solve_by_elim
 
-instance get_sound : Sound (Wlp.get (m := m) (σ := σ)) where
-  inter := by intros; simp_all [get, getThe,MonadStateOf.get, Wlp.get]
-  impl := by intros; simp_all [get, getThe,MonadStateOf.get,Wlp.get]
+instance get_sound : Sound (Wp.get (m := m) (σ := σ)) where
+  inter := by intros; simp_all [get, getThe,MonadStateOf.get, Wp.get]
+  impl := by intros; simp_all [get, getThe,MonadStateOf.get,Wp.get]
   -- call := by solve_by_elim
 
-instance set_sound (s : σ) : Sound (Wlp.set s (m := m)) where
-  inter := by intros; simp_all [Wlp.set]
-  impl := by intros; simp_all [Wlp.set]
+instance set_sound (s : σ) : Sound (Wp.set s (m := m)) where
+  inter := by intros; simp_all [Wp.set]
+  impl := by intros; simp_all [Wp.set]
   -- call := by solve_by_elim
 
-instance modifyGet_sound : Sound (Wlp.modifyGet f (m := m) (σ := σ) (ρ := ρ)) where
-  inter := by intros; simp_all [Wlp.modifyGet]
-  impl := by intros; simp_all [Wlp.modifyGet]
+instance modifyGet_sound : Sound (Wp.modifyGet f (m := m) (σ := σ) (ρ := ρ)) where
+  inter := by intros; simp_all [Wp.modifyGet]
+  impl := by intros; simp_all [Wp.modifyGet]
   -- call := by solve_by_elim
 
 instance if_sound [Decidable c] [instT: Sound t] [instS : Sound e] : Sound (ite c t e) where
@@ -424,13 +424,13 @@ instance if_sound [Decidable c] [instT: Sound t] [instS : Sound e] : Sound (ite 
   impl := by
     intros; by_cases c <;> simp_all <;> solve_by_elim [instT.impl, instS.impl]
 
-instance (act : Wlp m σ ρ) [IsSubStateOf σ σ'] [Sound act] :
+instance (act : Wp m σ ρ) [IsSubStateOf σ σ'] [Sound act] :
   Sound (act.lift (σ' := σ')) where
   inter := by
-    intros; simp_all [Wlp.lift]
+    intros; simp_all [Wp.lift]
     solve_by_elim [Sound.inter]
   impl := by
-    intros; simp_all [Wlp.lift]
+    intros; simp_all [Wp.lift]
     solve_by_elim [Sound.impl]
   -- call := by
   --   intros; simp_all [monadLift, MonadLift.monadLift]
@@ -438,13 +438,13 @@ instance (act : Wlp m σ ρ) [IsSubStateOf σ σ'] [Sound act] :
 
 /-! ### Correctness of `checkSpec` -/
 
-theorem wlp_spec_to_big_step :
-  (Wlp.spec ens req).toBigStep (m := .internal) = BigStep.spec ens req := by
-  ext s r' s'; unfold Wlp.spec BigStep.spec Wlp.toBigStep; simp
+theorem wp_spec_to_big_step :
+  (Wp.spec ens req).toBigStep (m := .internal) = BigStep.spec ens req := by
+  ext s r' s'; unfold Wp.spec BigStep.spec Wp.toBigStep; simp
 
 theorem check_spec_sound [Sound act] (req : SProp σ) (ens : σ -> RProp σ ρ) :
   (∀ s, req s -> act s (ens s)) ->
-  Wlp.spec (m := .internal) req ens <= act := by
+  Wp.spec (m := .internal) req ens <= act := by
   intro triple s post; simp [actSimp]; intros hreq hens
   solve_by_elim [Sound.impl]
 
